LogicGenerator/demo932/Interface.v
@@ -29,6 +29,9 @@ End PrimitiveRuleSig.
 Module Type LogicTheoremSig (Names: LanguageSig) (Rules: PrimitiveRuleSig Names).
 Include Rules.
 Parameter Inline tree_pos : Type .
+  Axiom sepcon_comm_impp : (forall x y : expr, provable (impp (sepcon x y) (sepcon y x))) .
+  Axiom sepcon_assoc1 : (forall x y z : expr, provable (impp (sepcon x (sepcon y z)) (sepcon (sepcon x y) z))) .
+  Axiom sepcon_mono : (forall x1 x2 y1 y2 : expr, provable (impp x1 x2) -> provable (impp y1 y2) -> provable (impp (sepcon x1 y1) (sepcon x2 y2))) .
   Axiom logic_equiv_derivable1 : (forall x y : expr, logic_equiv x y <-> derivable1 x y /\ derivable1 y x) .
   Axiom derivable1_sepcon_comm : (forall x y : expr, derivable1 (sepcon x y) (sepcon y x)) .
   Axiom derivable1_sepcon_assoc1 : (forall x y z : expr, derivable1 (sepcon x (sepcon y z)) (sepcon (sepcon x y) z)) .
@@ -102,9 +105,12 @@ Include Rules.
   Instance GammaEP : (EquivProvable L GammaP GammaE) := Provable2Equiv_Normal .
   Instance GammaD1P : (Derivable1Provable L GammaP GammaD1) := Provable2Derivable1_Normal .
   Instance GammaED1 : (EquivDerivable1 L GammaD1 GammaE) := Axiomatization2Deduction_GammaED1 .
-  Instance sepconAX : (SepconAxiomatization L GammaP) := SeparationAlgebra2SepconAxiomatization .
+  Instance (Pred_sepconAX model) : (SepconAxiomatization (PredicateAsLang.Pred_L model) (PredicatePropositionalLogic.Pred_Gamma model)) := SeparationAlgebra2SepconAxiomatization .
   Instance sepconD : (SepconDeduction L GammaD1) := SeparationLogic.Axiomatization2Deduction_sepconD .
 Definition tree_pos : Type := tree_pos.
+  Definition sepcon_comm_impp : (forall x y : expr, provable (impp (sepcon x y) (sepcon y x))) := sepcon_comm_impp .
+  Definition sepcon_assoc1 : (forall x y z : expr, provable (impp (sepcon x (sepcon y z)) (sepcon (sepcon x y) z))) := sepcon_assoc1 .
+  Definition sepcon_mono : (forall x1 x2 y1 y2 : expr, provable (impp x1 x2) -> provable (impp y1 y2) -> provable (impp (sepcon x1 y1) (sepcon x2 y2))) := sepcon_mono .
   Definition logic_equiv_derivable1 : (forall x y : expr, logic_equiv x y <-> derivable1 x y /\ derivable1 y x) := logic_equiv_derivable1 .
   Definition derivable1_sepcon_comm : (forall x y : expr, derivable1 (sepcon x y) (sepcon y x)) := derivable1_sepcon_comm .
   Definition derivable1_sepcon_assoc1 : (forall x y z : expr, derivable1 (sepcon x (sepcon y z)) (sepcon (sepcon x y) z)) := derivable1_sepcon_assoc1 .
